sfi/common.v
@@ -1,8 +1,6 @@
-Require Import eqtype.
+Require Import ssreflect ssrfun ssrbool eqtype ssrnat seq.
 Require Import lib.utils lib.partial_maps lib.ordered common.common.
 Set Bullet Behavior "Strict Subproofs".
-
-Section WithClasses.
 
 Generalizable All Variables.
 
@@ -25,4 +23,18 @@ Class sfi_syscall_addrs (t : machine_types) := {
   add_to_shared_memory_addr : word t
 }.
 
-End WithClasses.
+Inductive where_from :=
+| INTERNAL : where_from
+| JUMPED   : where_from.
+
+Definition where_from_eq (S1 S2 : where_from) : bool :=
+  match S1, S2 with
+    | INTERNAL , INTERNAL | JUMPED , JUMPED => true
+    | _ , _                                 => false
+  end.
+
+Lemma where_from_eqP : Equality.axiom where_from_eq.
+Proof. by move=> [|] [|] /=; apply: (iffP idP). Qed.
+
+Definition where_from_eqMixin := EqMixin where_from_eqP.
+Canonical where_from_eqType := Eval hnf in EqType where_from where_from_eqMixin.
