sfi/symbolic.v
@@ -4,16 +4,12 @@ Require Import ssreflect ssrfun ssrbool eqtype ssrnat seq.
 
 Require Import lib.utils lib.ordered lib.partial_maps common.common.
 Require Import symbolic.symbolic symbolic.rules.
-Require Import sfi.classes sfi.list_utils sfi.set_utils sfi.isolate_sets
+Require Import sfi.common sfi.list_utils sfi.set_utils sfi.isolate_sets
                sfi.ranges.
 
 Set Bullet Behavior "Strict Subproofs".
 
 Module Sym.
-
-Inductive where_from :=
-| INTERNAL : where_from
-| JUMPED   : where_from.
 
 Inductive stag {t : machine_types} :=
 | PC     : forall (S : where_from) (c : word t), stag
@@ -121,18 +117,6 @@ Definition stag_incoming (L : stag) : option (list (word t)) :=
 
 Definition stag_writers (L : stag) : option (list (word t)) :=
   match L with DATA _ _ W => Some W | _ => None end.
-
-Definition where_from_eq (S1 S2 : where_from) : bool :=
-  match S1, S2 with
-    | INTERNAL , INTERNAL | JUMPED , JUMPED => true
-    | _ , _                                 => false
-  end.
-
-Lemma where_from_eqP : Equality.axiom where_from_eq.
-Proof. by move=> [|] [|] /=; apply: (iffP idP). Qed.
-
-Definition where_from_eqMixin := EqMixin where_from_eqP.
-Canonical where_from_eqType := Eval hnf in EqType where_from where_from_eqMixin.
 
 Definition stag_eq (t1 t2 : stag) : bool :=
   match t1, t2 with
